sir/Sir/Vars/Proofs/Quotient.lean
@@ -1,0 +1,25 @@
+import Sir.Vars.Spec.Quotient
+
+namespace Sir.Vars.Proofs
+
+private def canonicalProgramEquivalenceClass :
+    { program : Program // program.Canonical } → Quotient Program.alphaEquivalenceSetoid :=
+  fun program => Quotient.mk Program.alphaEquivalenceSetoid program
+
+private theorem canonicalProgramEquivalenceClass_leftInverse :
+    Function.LeftInverse canonicalProgramEquivalenceClass
+      Program.canonicalizeEquivalenceClass := by
+  intro equivalenceClass
+  refine Quotient.inductionOn equivalenceClass ?_
+  intro program
+  exact Quotient.sound (Program.canonicalize_alphaEquiv program)
+
+theorem Program.canonicalizeEquivalenceClass_bijective :
+    Function.Bijective Vars.Program.canonicalizeEquivalenceClass := by
+  constructor
+  · exact canonicalProgramEquivalenceClass_leftInverse.injective
+  · intro program
+    refine ⟨canonicalProgramEquivalenceClass program, ?_⟩
+    exact Subtype.ext program.property
+
+end Sir.Vars.Proofs
