sir/Sir/Vars/Spec/Quotient.lean
@@ -1,0 +1,19 @@
+import Sir.Vars.Proofs.Canonical
+
+namespace Sir.Vars
+
+instance Program.alphaEquivalenceSetoid : Setoid Program where
+  r := Program.AlphaEquiv
+  iseqv := {
+    refl := Program.AlphaEquiv.refl
+    symm := Program.AlphaEquiv.symm
+    trans := Program.AlphaEquiv.trans }
+
+def Program.canonicalizeEquivalenceClass :
+    Quotient Program.alphaEquivalenceSetoid → { program : Program // program.Canonical } :=
+  Quotient.lift
+    (fun program => ⟨program.canonicalize, Program.canonicalize_canonical program⟩)
+    (fun _ _ equivalent =>
+      Subtype.ext (Program.alphaEquiv_iff_canonicalize_eq.mp equivalent))
+
+end Sir.Vars
